AutomataTheory/Automata/Sum.lean
@@ -116,8 +116,8 @@ variable {I A : Type*} (M : I → Automaton A) (acc : (i : I) → Set ((M i).Sta
 def Automaton.Sum_Acc : Set (Automaton.Sum M).State := ⋃ i : I, Sigma.mk i '' acc i
 
 theorem accepted_lang_union :
-    AcceptedLang (Automaton.Sum M) (Automaton.Sum_Acc M acc) = ⋃ i : I, AcceptedLang (M i) (acc i) := by
-  ext al ; simp [Automaton.Sum_Acc, AcceptedLang, FinAccept]
+    (Automaton.Sum M).AcceptedLang (Automaton.Sum_Acc M acc) = ⋃ i : I, (M i).AcceptedLang (acc i) := by
+  ext al ; simp [Automaton.Sum_Acc, Automaton.AcceptedLang, FinAccept]
   constructor
   · rintro ⟨n, as, ⟨ss, h_run, h_acc⟩, h_al⟩
     obtain ⟨i, ss_i, h_run_i, h_ss_i⟩ := automata_sum_fin_run.mp h_run
